iris/KernelDecode00.v
@@ -437,6 +437,11 @@ Lemma kd_d67fe0ef s : register_lookup misa (sregs s) = MISA_C -> cfg_ok s ->
   = Some (JAL (mword_of_int 2092390 : mword 21, Regidx (mword_of_int 1)), s).
 Proof. decode_bridge_ms. Qed.
 
+Lemma kd_e21ff0ef s : register_lookup misa (sregs s) = MISA_C -> cfg_ok s ->
+  exec (ext_decode (mword_of_int 0xe21ff0ef : mword 32) : M instruction) s
+  = Some (JAL (mword_of_int 2096672 : mword 21, Regidx (mword_of_int 1)), s).
+Proof. decode_bridge_ms. Qed.
+
 Lemma kd_eadfe0ef s : register_lookup misa (sregs s) = MISA_C -> cfg_ok s ->
   exec (ext_decode (mword_of_int 0xeadfe0ef : mword 32) : M instruction) s
   = Some (JAL (mword_of_int 2092716 : mword 21, Regidx (mword_of_int 1)), s).
