iris/KernelDecode02.v
@@ -182,6 +182,11 @@ Lemma kd_d57d s : eq_vec (_get_Misa_C (register_lookup misa s.(sregs))) ('b"1") 
   = Some (C_BEQZ (mword_of_int 247, Cregidx (mword_of_int 2)), s).
 Proof. intro H. rvc_oneshot s H. Qed.
 
+Lemma kd_dde5 s : eq_vec (_get_Misa_C (register_lookup misa s.(sregs))) ('b"1") = true ->
+  exec (ext_decode_compressed (mword_of_int 0xdde5 : mword 16)) s
+  = Some (C_BEQZ (mword_of_int 252, Cregidx (mword_of_int 3)), s).
+Proof. intro H. rvc_oneshot s H. Qed.
+
 Lemma kd_e4b8 s : eq_vec (_get_Misa_C (register_lookup misa s.(sregs))) ('b"1") = true ->
   exec (ext_decode_compressed (mword_of_int 0xe4b8 : mword 16)) s
   = Some (C_SD (mword_of_int 9, Cregidx (mword_of_int 1), Cregidx (mword_of_int 6)), s).
