iris/KernelDecode04.v
@@ -267,6 +267,11 @@ Lemma kd_04faf863 s : register_lookup misa (sregs s) = MISA_C -> cfg_ok s ->
   = Some (BTYPE (mword_of_int 80 : mword 13, Regidx (mword_of_int 15), Regidx (mword_of_int 21), BGEU), s).
 Proof. decode_bridge_ms. Qed.
 
+Lemma kd_05850493 s : register_lookup misa (sregs s) = MISA_C -> cfg_ok s ->
+  exec (ext_decode (mword_of_int 0x05850493 : mword 32) : M instruction) s
+  = Some (ITYPE (mword_of_int 88 : mword 12, Regidx (mword_of_int 10), Regidx (mword_of_int 9), ADDI), s).
+Proof. decode_bridge_ms. Qed.
+
 Lemma kd_0ad72023 s : register_lookup misa (sregs s) = MISA_C -> cfg_ok s ->
   exec (ext_decode (mword_of_int 0x0ad72023 : mword 32) : M instruction) s
   = Some (STORE (mword_of_int 160 : mword 12, Regidx (mword_of_int 13), Regidx (mword_of_int 14), 4), s).
