iris/KernelDecode05.v
@@ -298,6 +298,11 @@ Lemma kd_04f70863 s : register_lookup misa (sregs s) = MISA_C -> cfg_ok s ->
   = Some (BTYPE (mword_of_int 80 : mword 13, Regidx (mword_of_int 15), Regidx (mword_of_int 14), BEQ), s).
 Proof. decode_bridge_ms. Qed.
 
+Lemma kd_05050493 s : register_lookup misa (sregs s) = MISA_C -> cfg_ok s ->
+  exec (ext_decode (mword_of_int 0x05050493 : mword 32) : M instruction) s
+  = Some (ITYPE (mword_of_int 80 : mword 12, Regidx (mword_of_int 10), Regidx (mword_of_int 9), ADDI), s).
+Proof. decode_bridge_ms. Qed.
+
 Lemma kd_0607c863 s : register_lookup misa (sregs s) = MISA_C -> cfg_ok s ->
   exec (ext_decode (mword_of_int 0x0607c863 : mword 32) : M instruction) s
   = Some (BTYPE (mword_of_int 112 : mword 13, zreg, Regidx (mword_of_int 15), BLT), s).
