iris/KernelDecode06.v
@@ -17,6 +17,11 @@ Require Import WpRvcBridge.
 Local Open Scope Z_scope.
 Import Defs.
 
+Lemma kd_0491 s : eq_vec (_get_Misa_C (register_lookup misa s.(sregs))) ('b"1") = true ->
+  exec (ext_decode_compressed (mword_of_int 0x0491 : mword 16)) s
+  = Some (C_ADDI (mword_of_int 4, Regidx (mword_of_int 9)), s).
+Proof. intro H. rvc_oneshot s H. Qed.
+
 Lemma kd_00000717 s : register_lookup misa (sregs s) = MISA_C -> cfg_ok s ->
   exec (ext_decode (mword_of_int 0x00000717 : mword 32) : M instruction) s
   = Some (UTYPE (mword_of_int 0 : mword 20, Regidx (mword_of_int 14), AUIPC), s).
