iris/KernelDecode10.v
@@ -317,6 +317,11 @@ Lemma kd_06f71463 s : register_lookup misa (sregs s) = MISA_C -> cfg_ok s ->
   = Some (BTYPE (mword_of_int 104 : mword 13, Regidx (mword_of_int 15), Regidx (mword_of_int 14), BNE), s).
 Proof. decode_bridge_ms. Qed.
 
+Lemma kd_08050913 s : register_lookup misa (sregs s) = MISA_C -> cfg_ok s ->
+  exec (ext_decode (mword_of_int 0x08050913 : mword 32) : M instruction) s
+  = Some (ITYPE (mword_of_int 128 : mword 12, Regidx (mword_of_int 10), Regidx (mword_of_int 18), ADDI), s).
+Proof. decode_bridge_ms. Qed.
+
 Lemma kd_08a92023 s : register_lookup misa (sregs s) = MISA_C -> cfg_ok s ->
   exec (ext_decode (mword_of_int 0x08a92023 : mword 32) : M instruction) s
   = Some (STORE (mword_of_int 128 : mword 12, Regidx (mword_of_int 10), Regidx (mword_of_int 18), 4), s).
@@ -362,6 +367,11 @@ Lemma kd_41450513 s : register_lookup misa (sregs s) = MISA_C -> cfg_ok s ->
   = Some (ITYPE (mword_of_int 1044 : mword 12, Regidx (mword_of_int 10), Regidx (mword_of_int 10), ADDI), s).
 Proof. decode_bridge_ms. Qed.
 
+Lemma kd_45850913 s : register_lookup misa (sregs s) = MISA_C -> cfg_ok s ->
+  exec (ext_decode (mword_of_int 0x45850913 : mword 32) : M instruction) s
+  = Some (ITYPE (mword_of_int 1112 : mword 12, Regidx (mword_of_int 10), Regidx (mword_of_int 18), ADDI), s).
+Proof. decode_bridge_ms. Qed.
+
 Lemma kd_8aafe0ef s : register_lookup misa (sregs s) = MISA_C -> cfg_ok s ->
   exec (ext_decode (mword_of_int 0x8aafe0ef : mword 32) : M instruction) s
   = Some (JAL (mword_of_int 2089130 : mword 21, Regidx (mword_of_int 1)), s).
@@ -375,6 +385,11 @@ Proof. decode_bridge_ms. Qed.
 Lemma kd_96eff0ef s : register_lookup misa (sregs s) = MISA_C -> cfg_ok s ->
   exec (ext_decode (mword_of_int 0x96eff0ef : mword 32) : M instruction) s
   = Some (JAL (mword_of_int 2093422 : mword 21, Regidx (mword_of_int 1)), s).
+Proof. decode_bridge_ms. Qed.
+
+Lemma kd_9e7ff0ef s : register_lookup misa (sregs s) = MISA_C -> cfg_ok s ->
+  exec (ext_decode (mword_of_int 0x9e7ff0ef : mword 32) : M instruction) s
+  = Some (JAL (mword_of_int 2095590 : mword 21, Regidx (mword_of_int 1)), s).
 Proof. decode_bridge_ms. Qed.
 
 Lemma kd_a3dfd0ef s : register_lookup misa (sregs s) = MISA_C -> cfg_ok s ->
