iris/KernelDecode14.v
@@ -322,6 +322,11 @@ Lemma kd_a2bfe0ef s : register_lookup misa (sregs s) = MISA_C -> cfg_ok s ->
   = Some (JAL (mword_of_int 2091562 : mword 21, Regidx (mword_of_int 1)), s).
 Proof. decode_bridge_ms. Qed.
 
+Lemma kd_a47ff0ef s : register_lookup misa (sregs s) = MISA_C -> cfg_ok s ->
+  exec (ext_decode (mword_of_int 0xa47ff0ef : mword 32) : M instruction) s
+  = Some (JAL (mword_of_int 2095686 : mword 21, Regidx (mword_of_int 1)), s).
+Proof. decode_bridge_ms. Qed.
+
 Lemma kd_a55ff0ef s : register_lookup misa (sregs s) = MISA_C -> cfg_ok s ->
   exec (ext_decode (mword_of_int 0xa55ff0ef : mword 32) : M instruction) s
   = Some (JAL (mword_of_int 2095700 : mword 21, Regidx (mword_of_int 1)), s).
