iris/KernelDecode16.v
@@ -142,6 +142,11 @@ Lemma kd_00078023 s : register_lookup misa (sregs s) = MISA_C -> cfg_ok s ->
   = Some (STORE (mword_of_int 0 : mword 12, zreg, Regidx (mword_of_int 15), 1), s).
 Proof. decode_bridge_ms. Qed.
 
+Lemma kd_0009a503 s : register_lookup misa (sregs s) = MISA_C -> cfg_ok s ->
+  exec (ext_decode (mword_of_int 0x0009a503 : mword 32) : M instruction) s
+  = Some (LOAD (mword_of_int 0 : mword 12, Regidx (mword_of_int 19), Regidx (mword_of_int 10), false, 4), s).
+Proof. decode_bridge_ms. Qed.
+
 Lemma kd_00279693 s : register_lookup misa (sregs s) = MISA_C -> cfg_ok s ->
   exec (ext_decode (mword_of_int 0x00279693 : mword 32) : M instruction) s
   = Some (SHIFTIOP (mword_of_int 2 : mword 6, Regidx (mword_of_int 15), Regidx (mword_of_int 13), SLLI), s).
@@ -290,6 +295,11 @@ Proof. decode_bridge_ms. Qed.
 Lemma kd_9f5ff0ef s : register_lookup misa (sregs s) = MISA_C -> cfg_ok s ->
   exec (ext_decode (mword_of_int 0x9f5ff0ef : mword 32) : M instruction) s
   = Some (JAL (mword_of_int 2095604 : mword 21, Regidx (mword_of_int 1)), s).
+Proof. decode_bridge_ms. Qed.
+
+Lemma kd_9fbff0ef s : register_lookup misa (sregs s) = MISA_C -> cfg_ok s ->
+  exec (ext_decode (mword_of_int 0x9fbff0ef : mword 32) : M instruction) s
+  = Some (JAL (mword_of_int 2095610 : mword 21, Regidx (mword_of_int 1)), s).
 Proof. decode_bridge_ms. Qed.
 
 Lemma kd_b92ff0ef s : register_lookup misa (sregs s) = MISA_C -> cfg_ok s ->
