iris/KernelDecode22.v
@@ -22,6 +22,16 @@ Lemma kd_05b1 s : eq_vec (_get_Misa_C (register_lookup misa s.(sregs))) ('b"1") 
   = Some (C_ADDI (mword_of_int 12, Regidx (mword_of_int 11)), s).
 Proof. intro H. rvc_oneshot s H. Qed.
 
+Lemma kd_408c s : eq_vec (_get_Misa_C (register_lookup misa s.(sregs))) ('b"1") = true ->
+  exec (ext_decode_compressed (mword_of_int 0x408c : mword 16)) s
+  = Some (C_LW (mword_of_int 0, Cregidx (mword_of_int 1), Cregidx (mword_of_int 3)), s).
+Proof. intro H. rvc_oneshot s H. Qed.
+
+Lemma ke_408c s :
+  exec (execute (C_LW (mword_of_int 0, Cregidx (mword_of_int 1), Cregidx (mword_of_int 3)))) s
+  = Some (ExecuteAs (LOAD (mword_of_int 0 : mword 12, Regidx (mword_of_int 9), Regidx (mword_of_int 11), false, 4)), s).
+Proof. apply exec_execute_C_LW_leaf; first [ apply bv_eq; vm_compute; reflexivity | vm_compute; reflexivity ]. Qed.
+
 Lemma kd_4481 s : eq_vec (_get_Misa_C (register_lookup misa s.(sregs))) ('b"1") = true ->
   exec (ext_decode_compressed (mword_of_int 0x4481 : mword 16)) s
   = Some (C_LI (mword_of_int 0, Regidx (mword_of_int 9)), s).
