iris/KernelDecode24.v
@@ -187,6 +187,11 @@ Lemma kd_e7b9 s : eq_vec (_get_Misa_C (register_lookup misa s.(sregs))) ('b"1") 
   = Some (C_BNEZ (mword_of_int 39, Cregidx (mword_of_int 7)), s).
 Proof. intro H. rvc_oneshot s H. Qed.
 
+Lemma kd_ed89 s : eq_vec (_get_Misa_C (register_lookup misa s.(sregs))) ('b"1") = true ->
+  exec (ext_decode_compressed (mword_of_int 0xed89 : mword 16)) s
+  = Some (C_BNEZ (mword_of_int 13, Cregidx (mword_of_int 3)), s).
+Proof. intro H. rvc_oneshot s H. Qed.
+
 Lemma kd_f052 s : eq_vec (_get_Misa_C (register_lookup misa s.(sregs))) ('b"1") = true ->
   exec (ext_decode_compressed (mword_of_int 0xf052 : mword 16)) s
   = Some (C_SDSP (mword_of_int 4, Regidx (mword_of_int 20)), s).
