iris/KernelDecode25.v
@@ -297,6 +297,11 @@ Lemma kd_06e79a63 s : register_lookup misa (sregs s) = MISA_C -> cfg_ok s ->
   = Some (BTYPE (mword_of_int 116 : mword 13, Regidx (mword_of_int 14), Regidx (mword_of_int 15), BNE), s).
 Proof. decode_bridge_ms. Qed.
 
+Lemma kd_0809a583 s : register_lookup misa (sregs s) = MISA_C -> cfg_ok s ->
+  exec (ext_decode (mword_of_int 0x0809a583 : mword 32) : M instruction) s
+  = Some (LOAD (mword_of_int 128 : mword 12, Regidx (mword_of_int 19), Regidx (mword_of_int 11), false, 4), s).
+Proof. decode_bridge_ms. Qed.
+
 Lemma kd_2207e793 s : register_lookup misa (sregs s) = MISA_C -> cfg_ok s ->
   exec (ext_decode (mword_of_int 0x2207e793 : mword 32) : M instruction) s
   = Some (ITYPE (mword_of_int 544 : mword 12, Regidx (mword_of_int 15), Regidx (mword_of_int 15), ORI), s).
