iris/KernelDecode28.v
@@ -342,6 +342,11 @@ Lemma kd_80060613 s : register_lookup misa (sregs s) = MISA_C -> cfg_ok s ->
   = Some (ITYPE (mword_of_int 2048 : mword 12, Regidx (mword_of_int 12), Regidx (mword_of_int 12), ADDI), s).
 Proof. decode_bridge_ms. Qed.
 
+Lemma kd_825ff0ef s : register_lookup misa (sregs s) = MISA_C -> cfg_ok s ->
+  exec (ext_decode (mword_of_int 0x825ff0ef : mword 32) : M instruction) s
+  = Some (JAL (mword_of_int 2095140 : mword 21, Regidx (mword_of_int 1)), s).
+Proof. decode_bridge_ms. Qed.
+
 Lemma kd_86248493 s : register_lookup misa (sregs s) = MISA_C -> cfg_ok s ->
   exec (ext_decode (mword_of_int 0x86248493 : mword 32) : M instruction) s
   = Some (ITYPE (mword_of_int 2146 : mword 12, Regidx (mword_of_int 9), Regidx (mword_of_int 9), ADDI), s).
